wip

src/ast.scala
@@ -88,4 +88,5 @@ object Syntax {
                           tm: Term, not: Option[Notation] = None) extends Command
   case class Theorem(id: Ident, args: List[BoundArg], ty: Typ, prf: Term) extends Command
   case class Rewrite(vars: List[Ident], lhs: Term, rhs: Term) extends Command
+
 }
